more work on IFC Type system and some examples

examples/relational/ifc_ts.fst
@@ -1,70 +1,86 @@
 (*--build-config
     options:--admit_fsi FStar.Set --z3timeout 15;
-    other-files:set.fsi heap.fst st.fst all.fst st2.fst
+    other-files:set.fsi heap.fst st.fst all.fst st2.fst noninterference.fst
   --*)
 
 module IFC
 
+(* We model a simple IFC Type system *)
 open FStar.Comp
 open FStar.Heap
 open FStar.Relational
 
+(****************************** Preliminaries ******************************)
+
 (* We model labels with different levels as integers *)
-type label = int
+
+
+(* A top label that is lower than all other lables *)
+let top = 1000
+
+(* A bottom label that is lower than all other lables *)
+let bot = - top
+
+type label = l:int{bot <= l /\ l <= top}
 
 (* Label of the attacker *)
 assume val alpha : label
-assume val bot : bot:label{forall (l:label). bot <= l}
 
-(* Labeling function (assigns a label to every reference) *)
+
+(* A global labeling function (assigns a label to every reference) *)
 assume val label_fun : ref int -> Tot label
 
 (* A reference can be observed bu the attacker if its label is not higher than
    alpha *)
 let attacker_observable x = label_fun x <= alpha
 
-type alpha_equiv (h1:double heap) = (forall (x:ref int). attacker_observable x 
+(* We have alpha equivalence when two heaps are equal for all references that
+  have a label <= alpha and thus are observable by the attacker *)
+type a_equiv (h1:double heap) = (forall (x:ref int). attacker_observable x 
                                                    ==> sel (R.l h1) x = sel (R.r h1) x) 
 
-(* typing jugdement  e : l *)
+(* Function to create new labeled references *)
+assume val new_labeled_int : l:label -> x:ref int{label_fun x = l}
+
+
+(**************************** Typing Judgements ****************************)
+
+(* typing judgement  e : l 
+   - Expressions do not modify the heap 
+   - If we have alpha equivalence on the input heaps, then the results must be
+     equal if the expression label is lower than or equal to alpha *)
 type ni_exp (l:label) =
               unit -> 
               ST2 (double int)
                   (requires (fun h2 -> True))
-                  (ensures  (fun h1 r h2 -> alpha_equiv h1
-                                          ==>(equal (R.l h1) (R.l h2)
-                                            /\equal (R.r h1) (R.r h2)
-                                            /\ (if l <= alpha then 
-                                                 R.l r = R.r r 
-                                               else 
-                                                 true))))
+                  (ensures  (fun h1 r h2 -> equal (R.l h1) (R.l h2)
+                                         /\ equal (R.r h1) (R.r h2)
+                                         /\ (a_equiv h1
+                                            ==> (if l <= alpha then 
+                                                  R.l r = R.r r 
+                                                else 
+                                                  true))))
 
-type com (l:label) = unit 
-                    -> ST unit 
-                       (requires (fun h -> True))
-                       (ensures  (fun h1 r h2 ->
-                                       (forall (y:ref int). 
-                                        label_fun y <= l 
-                                        ==> sel h1 y = sel h2 y)))
-
-
-(* typing jugdement  l |- c *)
+(* typing judgement  l |- c 
+   - references with a label below l are not modified
+   - alpha equivalence on input heaps implies alpha equivalence on output
+     heaps *)
 type ni_com (l:label) =
               unit -> 
               ST2 (double unit)
                   (requires (fun h2 -> True))
-                  (ensures  (fun h1 _ h2 -> alpha_equiv h1
-                                            ==> (alpha_equiv h2
-                                             /\ (forall (y:ref int). 
-                                                label_fun y <= l 
-                                                ==> sel (R.l h1) y = sel (R.l h2) y
-                                                 /\ sel (R.r h1) y = sel (R.r h2) y))))
+                  (ensures  (fun h1 _ h2 -> (forall (y:ref int). 
+                                              label_fun y < l 
+                                              ==> sel (R.l h1) y = sel (R.l h2) y
+                                               /\ sel (R.r h1) y = sel (R.r h2) y)
+                                         /\ (a_equiv h1 ==> a_equiv h2)))
 
-(*
-val test : l:label -> com l -> Tot (ni_com l)
-let test _ c = fun () -> compose2_self c (twice ())
-*)
+(* We define noninterference for a program as noninterference for commands with
+   the label bottom *)
+type ni = ni_com bot
 
+
+(*********************** Typing Rules for Expressions **********************)
 
 (* Subtyping rule for expression labels 
 
@@ -72,8 +88,8 @@ let test _ c = fun () -> compose2_self c (twice ())
          -----------------
              e : l2
 *)
-val sub_exp : l1:label -> l2:label{l1 <= l2} -> e1:(ni_exp l1) -> Tot (ni_exp l2)
-let sub_exp _ _ e1 = fun () -> e1 ()
+val sub_exp : l1:label -> l2:label{l1 <= l2} -> =e1:(ni_exp l1) -> Tot (ni_exp l2)
+let sub_exp _ _ e1 () = e1 ()
 
 (* Typing rule for dereferencing
 
@@ -81,19 +97,20 @@ let sub_exp _ _ e1 = fun () -> e1 ()
          ----------------
              !r : l
 *)
-val ref_exp : r:ref int 
+val deref_exp : r:ref int 
 (*            -> Tot (ni_exp (label_fun r)) *)
 (* This is the above line inlined due to bug #377 ... *)
-           -> Tot (unit -> ST2 (double int) 
-                           (requires (fun _ -> True))
-                  (ensures  (fun h1 res h2 -> alpha_equiv h1 
-                                          ==>(equal (R.l h1) (R.l h2)
-                                            /\equal (R.r h1) (R.r h2)
-                                            /\ (if (label_fun r) <= alpha then 
-                                                 R.l res = R.r res 
-                                               else 
-                                                 true)))))
-let ref_exp r = fun () -> compose2_self (fun () -> (!r)) (twice ())
+           -> unit 
+           -> ST2 (double int)
+                  (requires (fun h2 -> True))
+                  (ensures  (fun h1 res h2 -> equal (R.l h1) (R.l h2)
+                                           /\ equal (R.r h1) (R.r h2)
+                                           /\ (a_equiv h1
+                                              ==> (if (label_fun r) <= alpha then 
+                                                    R.l res = R.r res
+                                                  else 
+                                                  true))))
+let deref_exp r () = compose2_self read (twice r)
 
 (* Typing rule for Int constants
 
@@ -102,29 +119,32 @@ let ref_exp r = fun () -> compose2_self (fun () -> (!r)) (twice ())
          i : bot 
 *)
 val const_exp : int -> Tot (ni_exp bot)
-let const_exp i = fun () -> twice i
+let const_exp i () = twice i
 
-
-
-(* Typing rule for binary operators 
+(* Typing rule for binary operators (we write the rule only for "+", but other
+   binarry operators work analogously
  
           e1 : l   e2 : l 
           ---------------
            e1 + e2  : l2
 *)
-val expr : l:label -> e1:(ni_exp l) -> e2:(ni_exp l) 
+val bin_op_exp : l:label -> =e1:(ni_exp l) -> =e2:(ni_exp l) 
 (*            -> Tot (ni_exp l) *)
 (* This is the above line inlined due to bug #377 ... *)
-           -> Tot (unit -> ST2 (double int) 
-                           (requires (fun _ -> True))
-                  (ensures  (fun h1 r h2 -> alpha_equiv h1 
-                                          ==>(equal (R.l h1) (R.l h2)
-                                            /\equal (R.r h1) (R.r h2)
-                                            /\ (if l <= alpha then 
-                                                 R.l r = R.r r 
-                                               else 
-                                                 true)))))
-let expr _ e1 e2 = (fun () -> compose2_self (fun (a, b) -> a + b) (pair_rel (e1 ()) (e2 ())))
+           -> unit 
+           -> ST2 (double int)
+                  (requires (fun h2 -> True))
+                  (ensures  (fun h1 r h2 -> equal (R.l h1) (R.l h2)
+                                         /\ equal (R.r h1) (R.r h2)
+                                         /\ (a_equiv h1
+                                            ==> (if l <= alpha then 
+                                                  R.l r = R.r r 
+                                                else 
+                                                  true))))
+let bin_op_exp _ e1 e2 () = compose2_self (fun (a, b) -> a + b) (pair_rel (e1 ()) (e2 ()))
+
+
+(************************ Typing Rules for Commands ************************)
 
 (* Subtyping rule for commands
 
@@ -132,30 +152,26 @@ let expr _ e1 e2 = (fun () -> compose2_self (fun (a, b) -> a + b) (pair_rel (e1 
          ------------------
               l2 |- c 
 *)
-val sub_comp : l1 : label -> l2:label{l2 <= l1} -> c1:(ni_com l1) -> Tot (ni_com l2)
-let sub_comp _ _ c1 = fun () -> c1 () 
+val sub_com : l1 : label -> l2:label{l2 <= l1} -> =c1:(ni_com l1) -> Tot (ni_com l2)
+let sub_com _ _ c1 () = c1 () 
 
-
-(* Rule for assignment 
-         e : l'      label_fun(r) = l'      l' > l
+(* Typing rule for assignment 
+         e : l'      label_fun(r) = l'      l' >= l
          ------------------------------------------
                        l |- r := e 
 *)
-val assign : l:label -> l':label{l' > l} -> r:ref int{label_fun r = l'} -> e:ni_exp l' 
-       //      -> Tot (ni_com l)
+val assign_com : l:label -> l':label{l' >= l} -> r:ref int{label_fun r = l'} -> =e:ni_exp l' 
+(*              -> Tot (ni_com l) *)
 (* This is the above line inlined due to bug #377 ... *)
-       -> Tot (unit -> 
+          ->  unit -> 
               ST2 (double unit)
                   (requires (fun h2 -> True))
-                  (ensures  (fun h1 _ h2 -> alpha_equiv h1
-                                            ==> (alpha_equiv h2
-                                             /\ (forall (y:ref int). 
-                                                label_fun y <= l 
-                                                ==> sel (R.l h1) y = sel (R.l h2) y
-                                                 /\ sel (R.r h1) y = sel (R.r h2) y))))) 
-let assign _ _ r e = fun () -> compose2_self (fun x -> r := x) (e ())
-
-
+                  (ensures  (fun h1 _ h2 -> (forall (y:ref int). 
+                                              label_fun y < l 
+                                              ==> sel (R.l h1) y = sel (R.l h2) y
+                                               /\ sel (R.r h1) y = sel (R.r h2) y)
+                                         /\ (a_equiv h1 ==> a_equiv h2)))
+let assign_com _ _ r e () = compose2_self (write r) (e ())
 
 (* Sequencing rule for commands
 
@@ -163,86 +179,323 @@ let assign _ _ r e = fun () -> compose2_self (fun x -> r := x) (e ())
          ------------------
             l |- c1; c2 
 *)
-val seq : l:label -> c1:(ni_com l) -> c2:(ni_com l) 
+val seq_com : l:label -> =c1:(ni_com l) -> =c2:(ni_com l) 
 (*             -> Tot(ni_com l) *)
 (* This is the above line inlined due to bug #377 ... *)
-       -> Tot (unit -> 
+          ->  unit -> 
               ST2 (double unit)
                   (requires (fun h2 -> True))
-                  (ensures  (fun h1 _ h2 -> alpha_equiv h1
-                                            ==> (alpha_equiv h2
-                                             /\ (forall (y:ref int). 
-                                                label_fun y <= l 
-                                                ==> sel (R.l h1) y = sel (R.l h2) y
-                                                 /\ sel (R.r h1) y = sel (R.r h2) y))))) 
-let seq _ c1 c2 = (fun () -> let _ = c1 () in c2 ())
-
-
+                  (ensures  (fun h1 _ h2 -> (forall (y:ref int). 
+                                              label_fun y < l 
+                                              ==> sel (R.l h1) y = sel (R.l h2) y
+                                               /\ sel (R.r h1) y = sel (R.r h2) y)
+                                         /\ (a_equiv h1 ==> a_equiv h2)))
+let seq_com _ c1 c2 () = let _ = c1 () in c2 ()
 
 (* This is used for cross cases (TODO: is this sound?)*)
 assume val cross : #p:(heap2 -> heap2 -> Type) 
                 -> #q:(heap2 -> heap2 -> Type) 
                 -> =c1:(unit -> ST2 (double unit) (requires (fun h -> True)) (ensures (fun h1 _ h2 -> p h1 h2))) 
                 -> =c2:(unit -> ST2 (double unit) (requires (fun h -> True)) (ensures (fun h1 _ h2 -> q h1 h2))) 
-                -> ST2 (double unit) (requires (fun h -> True)) (ensures (fun h1 _ h2 -> (exists (h2l:heap) (h2r:heap). p h1 (R (R.l h2) (h2r)) 
-                                                                                                                     /\ q h1 (R h2l (R.r h2)) )))
+                -> ST2 (double unit) (requires (fun h -> True)) 
+                                     (ensures (fun h1 _ h2 -> (exists (h2l:heap) (h2r:heap). p h1 (R (R.l h2) (h2r)) 
+                                                                                          /\ q h1 (R h2l (R.r h2)))))
 
 (* Conditional rule for commands
 
-         e : l     l |- ct     l |- cf    
-         -----------------------------
-           l |- if e then ct else cf
+         e : l     l |- ct      l |- cf    
+         ------------------------------
+         l |- if e <> 0 then ct else cf
 *)
-val cond : l:label -> e:(ni_exp l) -> ct:(ni_com l) -> cf:(ni_com l) 
+  val cond : l:label -> =e:(ni_exp l) -> =ct:(ni_com l) -> =cf:(ni_com l) 
            -> Tot (ni_com l)
-let cond _ e ct cf = (fun () -> match e () with 
-                     | R 0 0 -> cf ()
-                     | R 0 _ -> cross cf ct
-                     | R _ 0 -> cross ct cf 
-                     | R _ _ -> ct ())
+let cond _ e ct cf ()  = match e () with 
+                         | R 0 0 -> cf ()
+                         | R 0 _ -> cross cf ct
+                         | R _ 0 -> cross ct cf 
+                         | R _ _ -> ct ()
 
+(* Typing rule for Skip
 
-
-
-val skip : unit -> ST2 (double unit) (requires (fun h -> True)) (ensures (fun h1 _ h2 -> equal (R.l h1) (R.l h2) /\ equal (R.r h1) (R.r h2)))
+         -----------
+         top |- skip
+*)
+val skip : ni_com top
 let skip () = twice ()
 
-val loop_loop : l:label -> e:(ni_exp l) -> c:(ni_com l) 
-     //  -> Tot (ni_com l)
+(* Loop case of a while loop *)
+val loop_loop : l:label -> =e:(ni_exp l) -> =c:(ni_com l) 
+(*        -> Tot (ni_com l) *)
 (* This fails because of bug #379 *)
-       -> unit -> 
+           -> unit -> 
               ST2 (double unit)
                   (requires (fun h2 -> True))
-                  (ensures  (fun h1 _ h2 -> alpha_equiv h1
-                                            ==> (alpha_equiv h2
-                                             /\ (forall (y:ref int). 
-                                                label_fun y <= l 
-                                                ==> sel (R.l h1) y = sel (R.l h2) y
-                                                 /\ sel (R.r h1) y = sel (R.r h2) y))))
+                  (ensures  (fun h1 _ h2 -> (forall (y:ref int). 
+                                              label_fun y < l 
+                                              ==> sel (R.l h1) y = sel (R.l h2) y
+                                               /\ sel (R.r h1) y = sel (R.r h2) y)
+                                         /\ (a_equiv h1 ==> a_equiv h2)))
 
 (* While rule for commands
 
-         e : l        l |- c
-         -------------------
-         l |- wihle e do {c}
+         e : l               l |- c
+         --------------------------
+         l |- while (e <> 0) do {c}
 *)
-val loop : l:label -> e:(ni_exp l) -> c:(ni_com l) 
-          // -> Tot (ni_com l)
+val loop_com : l:label -> =e:(ni_exp l) -> =c:(ni_com l) 
+(*            -> Tot (ni_com l) *)
 (* This fails because of bug #379 *)
-       -> unit -> 
+           -> unit -> 
               ST2 (double unit)
                   (requires (fun h2 -> True))
-                  (ensures  (fun h1 _ h2 -> alpha_equiv h1
-                                            ==> (alpha_equiv h2
-                                             /\ (forall (y:ref int). 
-                                                label_fun y <= l 
-                                                ==> sel (R.l h1) y = sel (R.l h2) y
-                                                 /\ sel (R.r h1) y = sel (R.r h2) y))))
-let rec loop l e c = 
-                (fun () -> match e () with 
-                 | R 0 0 -> twice ()
+                  (ensures  (fun h1 _ h2 -> (forall (y:ref int). 
+                                              label_fun y < l 
+                                              ==> sel (R.l h1) y = sel (R.l h2) y
+                                               /\ sel (R.r h1) y = sel (R.r h2) y)
+                                         /\ (a_equiv h1 ==> a_equiv h2)))
+let rec loop_com l e c () = 
+                  match e () with 
+                 | R 0 0 -> skip ()
                  | R 0 _ -> cross skip (loop_loop l e c)
                  | R _ 0 -> cross (loop_loop l e c) skip
-                 | R _ _ -> loop_loop l e c ())
-and loop_loop l e c = fun () -> let _ = c () in loop l e c ()
+                 | R _ _ -> loop_loop l e c ()
+and loop_loop l e c () = let _ = c () in loop_com l e c ()
 
+
+
+(****************************** IFC_Examples ******************************)
+
+module IFC_Example1 
+open Distinct 
+open IFC
+open FStar.Comp
+open FStar.Relational
+
+(* Fails iff label b > label a *)
+let a = new_labeled_int 1
+let b = new_labeled_int 0
+
+assume Distinct : distinct2 a b
+
+let test () = (if !b <> 0 then
+                 a := 1
+               else
+                 a := 2);
+               b := 0
+
+(* Brute Force Approach *)
+val test_ni : ni
+let test_ni _ = compose2_self test (twice ())
+
+(* Following the typing derivation *)
+
+(* !b : 0 *)
+val ni_exp_deref_b : ni_exp 0
+let ni_exp_deref_b () = (deref_exp b) ()
+
+(* 1 : bot *)
+val ni_exp_1 : ni_exp bot
+let ni_exp_1 () = (const_exp 1) ()
+
+(* 1 : 1 *)
+val ni_exp_1' : ni_exp 1
+let ni_exp_1' = sub_exp bot 1 ni_exp_1
+
+(* 0 |- a := 1 *)
+val ni_com_a_1: ni_com 0
+let ni_com_a_1 () = (assign_com 0 1 a ni_exp_1') ()
+
+(* 2 : bot *)
+val ni_exp_2 : ni_exp bot
+let ni_exp_2 () = (const_exp  2) ()
+
+(* 2 : 1 *)
+val ni_exp_2' : ni_exp 1
+let ni_exp_2' = sub_exp bot 1 ni_exp_2
+
+(* 0 |- a := 2 *)
+val ni_com_a_2: ni_com 0
+let ni_com_a_2 () = (assign_com 0 1 a ni_exp_2') ()
+
+(* 0 |- if (!b <> 0) then a := 1 else a := 2 *)
+val ni_com_cond : ni_com 0 
+let ni_com_cond = cond 0 ni_exp_deref_b ni_com_a_1 ni_com_a_2
+
+(* bot |- if (!b <> 0) then a := 1 else a := 2 *)
+val ni_com_cond' : ni_com bot
+let ni_com_cond' = sub_com 0 bot ni_com_cond
+
+(* 2 : bot *)
+val ni_exp_0 : ni_exp bot
+let ni_exp_0 () = (const_exp 0) ()
+
+(* 2 : 0 *)
+val ni_exp_0' : ni_exp 0
+let ni_exp_0' = sub_exp bot 0 ni_exp_0
+
+(* bot |- b := 0 *)
+val ni_com_b : ni_com bot
+let ni_com_b () = (assign_com bot 0 b ni_exp_0') ()
+
+(* bot |- if (!b <> 0) then a := 1 else a := 2; b := 0 *)
+val ni_com_seq : ni_com bot
+let ni_com_seq () = (seq_com bot ni_com_cond' ni_com_b) ()
+
+(* Noninterference result for the complete program *)
+val ni_programm : ni
+let ni_programm () = ni_com_seq ()
+
+
+
+module IFC_Example3
+open IFC
+open FStar.Comp
+open FStar.Relational
+open Distinct
+
+assume val la : label
+assume val lb : lb:label{lb <= la}
+assume val lc : lc:label{lc <= la}
+
+let a = new_labeled_int la
+let b = new_labeled_int lb
+let c = new_labeled_int lc
+
+assume Distinct : distinct3 a b c
+
+let test () = a:= !b + !c
+
+(* Brute Force Approach *)
+val test_ni : ni
+let test_ni _ = compose2_self test (twice ())
+
+(* Following the typing derivation *)
+
+(* !b : lb *)
+val ni_exp_deref_b : ni_exp lb
+let ni_exp_deref_b () = (deref_exp b) ()
+
+(* !b : la *)
+val ni_exp_deref_b' : ni_exp la
+let ni_exp_deref_b' () = (sub_exp lb la ni_exp_deref_b) ()
+
+(* !c : lc *)
+val ni_exp_deref_c : ni_exp lc
+let ni_exp_deref_c () = (deref_exp c) ()
+
+(* !c : la *)
+val ni_exp_deref_c' : ni_exp la
+let ni_exp_deref_c' () = (sub_exp lc la ni_exp_deref_c) ()
+
+(* !b + !c : la *)
+val ni_exp_a : ni_exp la
+let ni_exp_a () = (bin_op_exp la ni_exp_deref_b' ni_exp_deref_c') ()
+
+(* bot |- a := !b + !c *)
+val ni_com_a: ni_com bot 
+let ni_com_a () = (assign_com bot la a ni_exp_a) ()
+
+(* Noninterference result for the complete program *)
+val ni_program : ni
+let ni_program () = ni_com_a () 
+
+
+module IFC_Example5
+open IFC
+open FStar.Comp
+open FStar.Relational
+open FStar.Heap
+open Distinct
+
+assume val la : label
+assume val lb : lb:label{lb >= la}
+assume val lc : lc:label
+
+let a = new_labeled_int la
+let b = new_labeled_int lb
+let c = new_labeled_int lc
+
+assume Distinct : distinct3 a b c
+
+(* This val-declaration is necessary (otherwise: FStar does not infer ST, but ALL) *)
+val loop : unit -> ST unit (requires (fun _ -> True))
+                           (ensures  (fun h r h' -> ((sel h a) = 0 ==> equal h h')
+                                                 /\ ((sel h a) <> 0  ==> equal h' (upd (upd h b ((sel h b) + (sel h a))) a 0))))
+let rec loop () = if !a <> 0 then (a := !a + -1; b := !b + 1; loop ())
+
+let test () = loop ();
+              c := 0
+
+(* Brute Force Approach *)
+val test_ni : ni
+let test_ni _ = compose2_self test (twice ())
+
+(* Following the typing derivation *)
+
+(* !a : la *)
+val ni_exp_deref_a : ni_exp la
+let ni_exp_deref_a () = (deref_exp a) ()
+
+(* -1 : bot *)
+val ni_exp__1 : ni_exp bot
+let ni_exp__1 () = (const_exp (-1)) ()
+
+(* -1 : la *)
+val ni_exp__1a : ni_exp la
+let ni_exp__1a () = (sub_exp bot la ni_exp__1) ()
+
+(* !a + -1 : la *)
+val ni_exp_a : ni_exp la
+let ni_exp_a () = (bin_op_exp la ni_exp_deref_a ni_exp__1a) ()
+
+(* la |- a := !a + -1  *)
+val ni_com_a : ni_com la
+let ni_com_a () = (assign_com la la a ni_exp_a) ()
+
+(* !b : lb *)
+val ni_exp_deref_b : ni_exp lb
+let ni_exp_deref_b () = (deref_exp b) ()
+
+(* 1 : bot *)
+val ni_exp_1 : ni_exp bot
+let ni_exp_1 () = (const_exp 1) ()
+
+(* 1 : lb *)
+val ni_exp_1b : ni_exp lb
+let ni_exp_1b () = (sub_exp bot lb ni_exp_1) ()
+
+(* !b + 1 : lb *)
+val ni_exp_b : ni_exp lb
+let ni_exp_b () = (bin_op_exp lb ni_exp_deref_b ni_exp_1b) ()
+
+(* la |- !b + 1 *)
+val ni_com_b : ni_com la
+let ni_com_b () = (assign_com la lb b ni_exp_b) ()
+
+(* la |- a := !a + -1; b := !b + 1 *)
+val ni_com_loop_body : ni_com la
+let ni_com_loop_body () = (seq_com la ni_com_a ni_com_b) ()
+
+(* la |- while !a <> 0 {a := !a + -1; b := !b + 1} *)
+val ni_com_loop : ni_com la
+let ni_com_loop () = (loop_com la ni_exp_deref_a ni_com_loop_body) ()
+
+(* bot |- while !a <> 0 {a := !a + -1; b := !b + 1} *)
+val ni_com_loop' : ni_com bot
+let ni_com_loop' () = (sub_com la bot ni_com_loop) ()
+
+(* 0 : bot *)
+val ni_exp_0 : ni_exp bot
+let ni_exp_0 () = (const_exp 0) ()
+
+(* 0 : lc *)
+val ni_exp_0' : ni_exp lc
+let ni_exp_0' () = (sub_exp bot lc ni_exp_0) ()
+
+(* bot |- c := 0 *)
+val ni_com_c : ni_com bot
+let ni_com_c () = (assign_com bot lc c ni_exp_0') ()
+
+(* Noninterference for the complete program *)
+val ni_program : ni 
+let ni_program () = (seq_com bot ni_com_loop' ni_com_c) ()
